src/Narcissus/BaseFormats.v
@@ -1,0 +1,8 @@
+Require Export
+        Fiat.Narcissus.Formats.Base.SequenceFormat
+        Fiat.Narcissus.Formats.Base.FMapFormat
+        Fiat.Narcissus.Formats.Base.StrictTerminalFormat
+        Fiat.Narcissus.Formats.Base.LaxTerminalFormat
+        Fiat.Narcissus.Formats.Base.FixFormat
+        Fiat.Narcissus.Formats.Base.EnqueueFormat
+        Fiat.Narcissus.Formats.Base.UnionFormat.
