src/Narcissus/Formats.v
@@ -7,5 +7,4 @@ Require Export
         Fiat.Narcissus.Formats.SumTypeOpt
         Fiat.Narcissus.Formats.IPChecksum
         Fiat.Narcissus.Formats.WordOpt
-        Fiat.Narcissus.Formats.FixFormat
         Fiat.Narcissus.Formats.NatOpt.
