src/Narcissus/Formats/Base/EnqueueFormat.v
@@ -1,0 +1,67 @@
+Require Import
+        Coq.omega.Omega
+        Coq.Strings.String
+        Coq.Vectors.Vector.
+
+Require Import
+        Fiat.Computation
+        Fiat.Narcissus.Common.Specs.
+
+Section UnionFormat.
+
+  Context {S : Type}. (* Source Type *)
+  Context {T : Type}. (* Target Type *)
+  Context {cache : Cache}. (* State Type *)
+  Context {monoid : Monoid T}. (* T is a monoid *)
+  Context {queue : QueueMonoidOpt monoid S}. (* T has an enqueue operation *)
+
+  Definition Enqueue_Format
+    : FormatM S T :=
+    fun a env => ret (enqueue_opt a mempty, env).
+
+  Definition Enqueue_Decode
+    : DecodeM (S * T) T :=
+    fun t env =>
+      Ifopt dequeue_opt t as st Then Some (st, env) Else None.
+
+  Definition Enqueue_Encode
+    : EncodeM S T :=
+    fun a env => Some (enqueue_opt a mempty, env).
+
+  Lemma CorrectDecoder_Enqueue
+    : CorrectDecoder_simpl (Enqueue_Format (decode).
+  Proof.
+    unfold CorrectDecoder_simpl, FMap_Decode, FMap_Format in *; split; intros.
+    { repeat (apply_in_hyp @unfold_computes; destruct_ex; intuition).
+      pose proof (g_inverts_f  _ _ _ _ H3 H4).
+      rewrite <- unfold_computes in H3.
+      eapply H1 in H3; destruct_ex; intuition eauto.
+      eexists; rewrite H5; simpl; intuition eauto.
+      subst; eauto.
+    }
+    { apply_in_hyp DecodeBindOpt_inv; destruct_ex; intuition.
+      eapply H2 in H3; eauto; injections.
+      destruct_ex; eexists; intuition eauto.
+      apply unfold_computes.
+      eexists; intuition eauto.
+    }
+  Qed.
+
+End UnionFormat.
+
+Definition Restrict_Format
+           {S T : Type}
+           {cache : Cache}
+           (P : S -> Prop)
+           (format : FormatM S T)
+  := FMap_Format (fun s s' => s = s' /\ P s) format.
+
+Definition Projection_Format
+           {S S' T : Type}
+           {cache : Cache}
+           (f : S -> S')
+           (format : FormatM S' T)
+  : FormatM S T :=
+  FMap_Format (fun s' s => f s = s') format.
+
+Notation "f <$> format" := (FMap_Format f format) (at level 99) : format_scope.
