src/Narcissus/Formats/Base/FMapFormat.v
@@ -1,0 +1,74 @@
+Require Import
+        Coq.omega.Omega
+        Coq.Strings.String
+        Coq.Vectors.Vector.
+
+Require Import
+        Fiat.Computation
+        Fiat.Narcissus.Common.Specs.
+
+Section UnionFormat.
+
+  Context {S : Type}. (* Source Type *)
+  Context {T : Type}. (* Target Type *)
+  Context {cache : Cache}. (* State Type *)
+
+  Context {S' : Type}. (* Transformed Type *)
+  Variable f : S -> S' -> Prop. (* Transformation Relation *)
+
+  Definition FMap_Format
+             (format_a : FormatM S T)
+    : FormatM S' T :=
+    fun a' env benv' =>
+      exists a, computes_to (format_a a env) benv' /\ f a a'.
+
+  Variable g : S -> S'. (* Transformation Function *)
+
+  Definition FMap_Decode
+             (decode : DecodeM S T)
+    : DecodeM S' T  :=
+    fun b env => `(a, env') <- decode b env; Some (g a, env').
+
+  Lemma CorrectDecoder_FMap
+        (format : FormatM S T)
+        (decode : DecodeM S T)
+        (format_decode_corect : CorrectDecoder_simpl format decode)
+        (g_inverts_f : forall a a' env benv,
+            format a env benv -> f a a' -> g a = a')
+        (g_OK : forall a, f a (g a))
+    : CorrectDecoder_simpl (FMap_Format format) (FMap_Decode decode).
+  Proof.
+    unfold CorrectDecoder_simpl, FMap_Decode, FMap_Format in *; split; intros.
+    { repeat (apply_in_hyp @unfold_computes; destruct_ex; intuition).
+      pose proof (g_inverts_f  _ _ _ _ H3 H4).
+      rewrite <- unfold_computes in H3.
+      eapply H1 in H3; destruct_ex; intuition eauto.
+      eexists; rewrite H5; simpl; intuition eauto.
+      subst; eauto.
+    }
+    { apply_in_hyp DecodeBindOpt_inv; destruct_ex; intuition.
+      eapply H2 in H3; eauto; injections.
+      destruct_ex; eexists; intuition eauto.
+      apply unfold_computes.
+      eexists; intuition eauto.
+    }
+  Qed.
+
+End UnionFormat.
+
+Definition Restrict_Format
+           {S T : Type}
+           {cache : Cache}
+           (P : S -> Prop)
+           (format : FormatM S T)
+  := FMap_Format (fun s s' => s = s' /\ P s) format.
+
+Definition Projection_Format
+           {S S' T : Type}
+           {cache : Cache}
+           (f : S -> S')
+           (format : FormatM S' T)
+  : FormatM S T :=
+  FMap_Format (fun s' s => f s = s') format.
+
+Notation "f <$> format" := (FMap_Format f format) (at level 99) : format_scope.
