src/Narcissus/Formats/Base/FixFormat.v
@@ -1,0 +1,126 @@
+Require Import
+        Coq.omega.Omega
+        Coq.Strings.String
+        Coq.Vectors.Vector.
+
+Require Import
+        Fiat.Computation
+        Fiat.Narcissus.Common.Specs
+        Fiat.Narcissus.Formats.Base.FMapFormat.
+
+Require Import Fiat.Computation.FixComp.
+Import Fiat.Computation.FixComp.LeastFixedPointFun.
+
+Section FixFormat.
+
+  Context {S : Type}. (* Source Type *)
+  Context {T : Type}. (* Target Type *)
+  Context {cache : Cache}. (* State Type *)
+
+  Definition Fix_Format
+             (format_body : FormatM S T -> FormatM S T)
+    := LeastFixedPoint (fDom := [S; CacheFormat]%type)
+                       (fCod := T * CacheFormat) format_body.
+
+  sxFixpoint FueledFix' {A B C}
+           (f : (B -> C -> option A) -> B -> C -> option A)
+           (n : nat)
+    : B -> C -> option A :=
+    match n with
+    | Datatypes.S n' => f (FueledFix' f n')
+    | _ => fun _ _ => None
+    end.
+
+  Definition Fix_Decode
+             (decode_body : DecodeM S T -> DecodeM S T)
+    : nat -> DecodeM S T :=
+    FueledFix' decode_body.
+
+  Lemma CorrectDecoder_Fix
+        {monoid : Monoid T}
+        (format_body : FormatM S T -> FormatM S T)
+        (decode_body : DecodeM S T -> DecodeM S T)
+    : forall (sz : nat),
+      (forall s env tenv', computes_to (Fix_Format format_body s env) tenv'
+                          -> bin_measure (fst tenv') > 0)
+      -> (forall (sz' : nat),
+          sz' < sz ->
+          CorrectDecoder_simpl (fun s env tenv' => computes_to (Fix_Format format_body s env) tenv'
+                                                   /\ bin_measure (fst tenv') <= sz') (Fix_Decode decode_body sz'))
+      -> CorrectDecoder_simpl (Fix_Format format_body) (Fix_Decode decode_body sz).
+  Proof.
+    intros.
+    unfold Fix_Decode; simpl.
+    induction sz.
+    simpl; intros.
+
+
+  Lemma fix_format_correct_simpl''
+      {A B}
+      {cache : Cache}
+      {monoid : Monoid B}
+      (format_body : funType [A; CacheFormat]%type (B * CacheFormat) ->
+                     funType [A; CacheFormat]%type (B * CacheFormat))
+                     (decode_body : (B ->  CacheDecode -> option (A * CacheDecode)) ->
+                     B -> CacheDecode -> option (A * CacheDecode))
+      (format_body_OK : Frame.monotonic_function format_body)
+      (decode_body_correct :
+         forall (format : funType [A; CacheFormat]%type (B * CacheFormat)) decode,
+           (CorrectDecoder_simpl' format decode bin')
+           -> CorrectDecoder_simpl' (format_body format) (decode_body decode) bin)
+  : CorrectDecoder_simpl (LeastFixedPoint format_body)
+                         (FueledFix decode_body).
+Proof.
+  unfold CorrectDecoder_simpl.
+  assert (forall n bin, bin_measure bin < n ->
+          (forall (env : CacheFormat) (env' : CacheDecode) (xenv : CacheFormat) (data : A),
+    Equiv env env' ->
+    LeastFixedPoint format_body data env ↝ (bin, xenv) ->
+    exists xenv' : CacheDecode, FueledFix' decode_body n bin env' = Some (data, xenv') /\ Equiv xenv xenv') /\
+   (forall (env : CacheFormat) (env' xenv' : CacheDecode) (data : A),
+    Equiv env env' ->
+    FueledFix' decode_body n bin env' = Some (data, xenv') ->
+    exists xenv : CacheFormat, LeastFixedPoint format_body data env ↝ (bin, xenv) /\ Equiv xenv xenv'));
+  try (intuition eauto; eapply H; eauto).
+  intros ? ?.
+  specialize (decode_body_correct bin); revert bin decode_body_correct.
+  induction n.
+  intros; inversion H.
+  intros; pose proof (fun a b c d e f g => proj1  (decode_body_correct a b c) d e f g);
+    pose proof (fun a b c d e f g => proj2 (decode_body_correct a b c) d e f g).
+  clear decode_body_correct.
+  split.
+  intros.
+  eapply (unroll_LeastFixedPoint format_body_OK) in H3; eauto.
+  simpl; eapply H0; try eauto.
+  intros.
+  eapply
+  split.
+  intros; eapply IHn; eauto.
+  admit.
+  intros.
+  simpl in H3; eapply H0 in H3; eauto.
+  destruct_ex; eexists; intuition eauto.
+  eapply (unroll_LeastFixedPoint' format_body_OK); eauto.
+  admit.
+
+  destruct H3.
+  eexists.
+
+  intros; eapply H; eauto.
+  admit.
+
+  eapply (proj1 IHn).
+  split.
+
+
+  eapply (well_founded_ind well_founded_lt_b); intros.
+  split; intros.
+  -  rewrite Init.Wf.Fix_eq by eassumption.
+     eapply decode_body_correct; eauto.
+     eapply (unroll_LeastFixedPoint format_body_OK); eauto.
+  - rewrite Init.Wf.Fix_eq in H1 by eassumption.
+    eapply decode_body_correct in H1; eauto.
+    destruct_ex; eexists; intuition eauto.
+    eapply (unroll_LeastFixedPoint' format_body_OK); eauto.
+Qed.
