src/Narcissus/Formats/Base/StrictTerminalFormat.v
@@ -1,0 +1,68 @@
+Require Import
+        Coq.omega.Omega
+        Coq.Strings.String
+        Coq.Vectors.Vector.
+
+Require Import
+        Fiat.Computation
+        Fiat.Narcissus.Common.Specs.
+
+Section StrictTerminalFormat.
+
+  Context {S : Type}. (* Source type *)
+  Context {T : Type}. (* Target type *)
+  Context {cache : Cache}. (* State type *)
+  Context {monoid : Monoid T}. (* Target type is a monoid *)
+
+  Definition StrictTerminal_Format
+    : FormatM S T :=
+    fun a env =>
+      t <- {t | bin_measure t = 0};
+      ret (t, env).
+
+  Definition StrictTerminal_Decode
+             (s : S)
+    : DecodeM S T :=
+    fun t env =>
+      If (beq_nat (bin_measure t) 0)
+         Then Some (s, env)
+         Else None.
+
+  Definition StrictTerminal_Encode
+    : EncodeM S T :=
+    fun a env => Some (mempty, env).
+
+  Lemma CorrectDecoder_StrictTerminal
+        (s : S)
+        (Singleton_Format : forall s' env tenv',
+            computes_to (StrictTerminal_Format s env) tenv' ->
+            s = s')
+    : CorrectDecoder_simpl StrictTerminal_Format (StrictTerminal_Decode s).
+  Proof.
+    unfold CorrectDecoder_simpl, StrictTerminal_Decode, StrictTerminal_Format in *; split; intros.
+    { computes_to_inv; injections; subst.
+      rewrite H0; simpl.
+      eexists; intuition eauto.
+      erewrite Singleton_Format with (env := xenv); eauto.
+    }
+    { destruct (beq_nat (bin_measure bin) 0) eqn: ?; simpl in *;
+        try discriminate.
+      apply_in_hyp beq_nat_true.
+      injections.
+      eexists env; intuition eauto.
+    }
+  Qed.
+
+  Lemma CorrectEncoder_Enqueue
+    : CorrectEncoder StrictTerminal_Format StrictTerminal_Encode.
+  Proof.
+    unfold CorrectEncoder, StrictTerminal_Format, StrictTerminal_Encode;
+      split; intros.
+    -  injections;
+         repeat computes_to_econstructor; eauto using measure_mempty.
+    - discriminate.
+  Qed.
+
+End StrictTerminalFormat.
+
+Notation "'ϵ'" := (StrictTerminal_Format) (at level 99) : format_scope.
