src/Narcissus/Formats/Base/UnionFormat.v
@@ -1,0 +1,60 @@
+Require Import
+        Fiat.Common.ilist
+        Fiat.Common.IterateBoundedIndex
+        Fiat.Narcissus.Common.Specs.
+
+Require Import
+        Coq.Sets.Ensembles.
+
+Section UnionFormat.
+
+  Context {S : Type}. (* Source Type *)
+  Context {T : Type}. (* Target Type *)
+  Context {cache : Cache}. (* State Type *)
+
+  Definition Union_Format {m}
+             (formats : Vector.t (FormatM S T) m)
+    : FormatM S T :=
+    fun s env tenv' =>
+      exists idx, computes_to (Vector.nth formats idx s env) tenv'.
+
+  Definition Union_Decode
+             {m}
+             (decoders : Vector.t (DecodeM S T) m)
+             (idx : Fin.t m)
+    : DecodeM S T := Vector.nth decoders idx.
+
+  Definition Union_Encode
+             {m}
+             (encoders : Vector.t (EncodeM S T) m)
+             (idx : Fin.t m)
+    : EncodeM S T := Vector.nth encoders idx.
+
+  Lemma CorrectDecoder_Union {m}
+        (formats : Vector.t (FormatM S T) m)
+        (decoders : Vector.t (DecodeM S T) m)
+        (correct_decoders :
+           Iterate_Ensemble_BoundedIndex'
+             (fun idx =>
+                CorrectDecoder_simpl (Vector.nth formats idx) (Vector.nth decoders idx)))
+        (idx : Fin.t m)
+        (unique_format :
+           forall s env t env',
+             (computes_to (Union_Format formats s env) (t, env') ->
+              computes_to (Vector.nth formats idx s env) (t, env')))
+    : CorrectDecoder_simpl (Union_Format formats) (Union_Decode decoders idx).
+Proof.
+  unfold CorrectDecoder_simpl, Union_Decode, Union_Format in *; split; intros.
+  { eapply unique_format in H0.
+    eapply Iterate_Ensemble_equiv' in correct_decoders.
+    eapply correct_decoders in H0; eauto.
+  }
+  { eapply Iterate_Ensemble_equiv' in correct_decoders.
+    eapply correct_decoders in H0; eauto.
+    destruct_ex; intuition; eexists; split; eauto.
+    apply unfold_computes.
+    eexists; intuition eauto.
+  }
+Qed.
+
+End UnionFormat.
